@prefix dc: <http://dublincore.org/elements/1.1/> .
@prefix dcterms: <http://purl.org/dc/terms/> .
@prefix edUse: <http://purl.org/dcx/lrmi-vocabs/educationalUse/> .
@prefix rdf: <http://www.w3.org/1999/02/22-rdf-syntax-ns#> .
@prefix rdfs: <http://www.w3.org/2000/01/rdf-schema#> .
@prefix skos: <http://www.w3.org/2004/02/skos/core#> .
@prefix skosxl: <http://www.w3.org/2008/05/skos-xl#> .
@prefix xml: <http://www.w3.org/XML/1998/namespace> .
@prefix xsd: <http://www.w3.org/2001/XMLSchema#> .

edUse: a skos:ConceptScheme ;
    dc:title "LRMI Educational Use vocabulary" ;
    dc:creator "LRMI Task Group (DCMI)"@en-US ;
    dcterms:description "A concept scheme that enumerates the educational uses of a learning resource."@en-US ;
    dcterms:created "2017-03-01"^^xsd:date ;
    dcterms:modified "2017-07-11"^^xsd:date ;    
    skos:hasTopConcept edUse:assessment, edUse:instruction,
        edUse:professionalSupport ;
    dcterms:license <http://creativecommons.org/licenses/by/4.0/> .
    
edUse:assessment a skos:Concept ;
    skos:prefLabel "assessment"@en-US ;
    skos:definition "Primary purpose of the resource is to evaluate learning, before, during, or after instruction occurs."@en-US ;
    skos:inScheme edUse: ;
    dcterms:source "Based on Common Education Data Standards (CEDS): https://ceds.ed.gov/element/001002#Assessment"@en-US .           

edUse:instruction a skos:Concept ;
    skos:prefLabel "instruction"@en-US ;
    skos:definition "Primary purpose of the resource is to support the instructional process, student learning, or to provide information about the curriculum."@en-US ;
    skos:inScheme edUse: ;
    dcterms:source "Based on Common Education Data Standards (CEDS): https://ceds.ed.gov/element/001002#CurriculumInstruction"@en-US .  

edUse:professionalSupport a skos:Concept ;
    skos:prefLabel "professional support"@en-US ;
    skos:definition "Primary purpose of the resource is to provide instruction for a teacher or other education professional including porofessional development."@en-US ;
    skos:inScheme edUse: ;
    dcterms:source "Based on Common Education Data Standards (CEDS): https://ceds.ed.gov/element/001002#ProfessionalDevelopment"@en-US .
